Proved that the VM operations preserves the invariant

RegexCorrectness/VM/Path/VMPath.lean
@@ -1,9 +1,10 @@
+import Regex.Data.SparseSet
 import RegexCorrectness.VM.Path.EpsilonClosure
 import RegexCorrectness.VM.Path.CharStep
 
 set_option autoImplicit false
 
-open Regex.Data (Span)
+open Regex.Data (Span SparseSet Vec)
 open Regex (NFA)
 open String (Pos Iterator)
 
@@ -20,6 +21,22 @@ end Regex.NFA
 
 namespace Regex.VM
 
+structure SearchState' (nfa : NFA) where
+  states : SparseSet nfa.nodes.size
+  updates : Vec (List (Nat × Pos)) nfa.nodes.size
+
+/--
+As an optimization, we write the updates to the buffer only when the state is done, a character, or a sparse state.
+-/
+def WriteUpdate {nfa : NFA} (i : Fin nfa.nodes.size) : Prop :=
+  match nfa[i] with
+  | .done | .char _ _ | .sparse _ _ => True
+  | _ => False
+
+/--
+All states in `next.state` have a corresponding path from `nfa.start` to the state where the span
+ends at `it`, and their updates are written to `next.updates` when necessary.
+-/
 def SearchState'.Inv (nfa : NFA) (wf : nfa.WellFormed) (it : Iterator) (next : SearchState' nfa) : Prop :=
   ∀ i ∈ next.states,
     ∃ span update,
@@ -28,3 +45,7 @@ def SearchState'.Inv (nfa : NFA) (wf : nfa.WellFormed) (it : Iterator) (next : S
       (WriteUpdate i → next.updates[i] = update)
 
 end Regex.VM
+
+theorem Regex.NFA.CharStep.write_update {nfa : NFA} {l m c r i j}
+  (step : nfa.CharStep l m c r i j) : Regex.VM.WriteUpdate i := by
+  cases step <;> simp_all [VM.WriteUpdate]
