RegexCorrectness/VM/Search/Lemmas.lean
@@ -1,0 +1,11 @@
+import RegexCorrectness.VM.Search.Basic
+
+set_option autoImplicit false
+
+open Regex.Data (SparseSet Vec)
+open Regex (NFA)
+open String (Pos Iterator)
+
+namespace Regex.VM
+
+end Regex.VM
